Main.lean
@@ -6,5 +6,4 @@ def main : IO Unit := do
   let input : Array Int256 :=
     #[1, 2, 3, 4, 5].map (BitVec.ofNat 256)
   IO.println s!"input    : {input.toList.map BitVec.toNat}"
-  IO.println s!"impl xs  : {(impl input).toList.map BitVec.toNat}"
-  IO.println s!"spec xs  : {(reverseSpec input).map BitVec.toNat}"
+  IO.println s!"impl xs  : {(reverseImpl input).toList.map BitVec.toNat}"
